put raiseException and translate into an extended monad, so that we can write theorems which universally quantify over them, rather than just assuming the concrete implementation of the Haskell spec

src/Program.v
@@ -4,12 +4,24 @@ Require Import riscv.Utility.
 Require Import Coq.ZArith.BinInt.
 Require Import bbv.Word.
 
+Inductive AccessType: Set := Instr | Load | Store.
+
 Section Riscv.
 
   Context {Name: NameWithEq}. (* register name *)
-  Notation Register := (@name Name).
+  Let Register := @name Name.
 
-  Class RiscvState(M: Type -> Type){t: Set}{MW: MachineWidth t} := mkRiscvState {
+  (* monad (will be instantiated with some kind of state monad) *)
+  Context {M: Type -> Type}.
+  Context {MM: Monad M}.
+
+  (* type of register values *)
+  Context {t: Set}.
+
+  (* provides operations on t *)
+  Context {MW: MachineWidth t}.
+
+  Class RiscvProgram := mkRiscvProgram {
     getRegister: Register -> M t;
     setRegister: Register -> t -> M unit;
 
@@ -35,12 +47,42 @@ Section Riscv.
   }.
 
 
-  Definition raiseException{A: Type}{t: Set}{MW: MachineWidth t}{M: Type -> Type}
-    {MM: Monad M}{RVS: RiscvState M}
+  (* The Haskell spec defines concrete implementations for raiseException and translate,
+     but we prefer to leave them abstract, so that we can prove more general theorems *)
+  Class RiscvState{MP: RiscvProgram} := mkRiscvState {
+    (* ends current cycle, sets exception flag, and sets PC to exception handler address *)
+    raiseException{A: Type}(isInterrupt: t)(exceptionCode: t): M A;
+
+    (* checks that addr is aligned, and translates the (possibly virtual) addr to a physical
+       address, raising an exception if the address is invalid *)
+    translate(accessType: AccessType)(alignment: t)(addr: t): M t;
+  }.
+
+  Definition default_raiseException{A: Type}{MP: RiscvProgram}
     (isInterrupt: t)(exceptionCode: t): M A :=
     pc <- getPC;
     addr <- getCSRField_MTVecBase;
     setPC (fromImm (addr * 4)%Z);;
     endCycle.
 
+
+  Local Open Scope alu_scope.
+  Local Open Scope Z_scope.
+
+  (* in a system with virtual memory, this would also do the translation, but in our
+     case, we only verify the alignment *)
+  Definition default_translate{MP: RiscvProgram}
+    (accessType: AccessType)(alignment: t)(addr: t): M t :=
+    if rem addr alignment /= zero
+    then default_raiseException zero four
+    else Return addr.
+
+  Instance DefaultRiscvState{MP: RiscvProgram}: RiscvState := {|
+    raiseException A := default_raiseException;
+    translate := default_translate;
+  |}.
+
 End Riscv.
+
+Arguments RiscvProgram {Name} (M) (t).
+Arguments RiscvState {Name} (M) (t) {MP}.
