src/Example.v
@@ -79,7 +79,7 @@ Definition fib6_L_trace(fuel: nat): option (list TraceEvent) :=
 Transparent wlt_dec.
 
 (* only uncomment this if you're sure there are no admits in the computational parts,
-   otherwise this will eat all your memory *)
+   otherwise this will eat all your memory
 
 Eval cbv in (load_byte_list (initialRiscvMachine fib6_riscv).(machineMem) $0 40).
 
